{
 "cells": [
  {
   "cell_type": "markdown",
   "metadata": {},
   "source": [
    "<p style=\"font-size:25px;\">\n",
    "<b>Exercise 6.1</b> \n",
    "</p>\n",
    "\n",
    "If V changes during the episode, then (6.6) only holds approximately; what\n",
    "would the difference be between the two sides? Let $V_t$ denote the array of state values\n",
    "used at time t in the TD error (6.5) and in the TD update (6.2). Redo the derivation\n",
    "above to determine the additional amount that must be added to the sum of TD errors\n",
    "in order to equal the Monte Carlo error.\n",
    "\n",
    "<p style=\"font-size:22px;\">\n",
    "<b>Answer:</b> \n",
    "</p>"
   ]
  },
  {
   "cell_type": "markdown",
   "metadata": {},
   "source": [
    "$V_{t+1}(S_{t+1})$ is the same as $V_t(S_{t+1})$ in MC case, and most of the time in TD case. But when $S_{t+1} = S_t$ then, in TD, we update this value in the previous step (because of the TD error incremental update). Therefore, those two terms are not equal, and they differ by the value of the TD error: $\\alpha[R_{t+1} + \\gamma V_t(S_{t+1}) - V_t(S_t)]$\n",
    "\n",
    "Because of this, we have almost the same equations, except when $S_t = S_{t+1}$ when we need to account for the term above\n",
    "\n",
    "$V_{t+1}(S_t) = V_t(S_t) + \\alpha[R_{t+1} + \\gamma V_t(S_{t+1}) - V_t(S_t)] = V_t(S_t) + \\alpha \\delta_t$\n",
    "\n",
    "\n",
    "$G_t - V(S_t) = R_{t+1} + \\gamma G_{t+1} - V_t(S_t) = \\delta_t + \\gamma[G_{t+1} - V_t(S_{t+1})]$\n",
    "\n",
    "With what we said above: \n",
    "\n",
    "$V_t(S_{t+1}) = V_{t+1}(S_{t+1}) - \\alpha \\delta_t \\mathbb{1}(S_{t+1}=S_t)$ with $\\mathbb{1}$ being the indicator function\n",
    "\n",
    "Therefore, we have: \n",
    "\n",
    "$G_t - V_t(S_t) = \\delta_t + \\gamma \\alpha \\delta_t \\mathbb{1}(S_{t+1}=S_t) + \\gamma[G_{t+1} - V_{t+1}(S_{t+1})] = \\delta_t + \\gamma \\alpha \\delta_t \\mathbb{1}(S_{t+1}=S_t) + \\gamma[\\delta_{t+1} + \\gamma \\alpha \\delta_{t+1}\\mathbb{1}(S_{t+1}=S_t) + \\gamma(G_{t+2} - V_{t+2}(S_{t+2}))]$\n",
    "\n",
    "Finally: \n",
    "\n",
    "$G_t - V_t(S_t) = \\sum_{k=t}^{T-1}\\gamma^{k-t}\\delta_k + \\alpha \\gamma \\sum_{k=t}^{T-1}\\gamma^{k-t}\\delta_t\\mathbb{1}(S_{t+1}=S_t)$"
   ]
  },
  {
   "cell_type": "markdown",
   "metadata": {},
   "source": []
  },
  {
   "cell_type": "markdown",
   "metadata": {},
   "source": []
  }
 ],
 "metadata": {
  "language_info": {
   "name": "python"
  }
 },
 "nbformat": 4,
 "nbformat_minor": 2
}
